\documentclass{article}
\usepackage{bussproofs}
\usepackage[landscape, margin=1cm]{geometry}
\begin{document}
\noindent Here is a derivation of: $\lambda$\textit{x}:(A$\times$B).\{(snd \textit{x}),(fst \textit{x})\}:((A$\times$B)$\to$(B$\times$A))
\begin{prooftree}\RightLabel{{\small Ax}}
\AxiomC{$\Gamma$, \textit{x}:(A$\times$B) $\vdash$ \textit{x}:(A$\times$B)}
\RightLabel{{\small $\times$Elim1}}
\UnaryInfC{$\Gamma$, \textit{x}:(A$\times$B) $\vdash$ (fst \textit{x}):A}
\RightLabel{{\small Ax}}
\AxiomC{$\Gamma$, \textit{x}:(A$\times$B) $\vdash$ \textit{x}:(A$\times$B)}
\RightLabel{{\small $\times$Elim2}}
\UnaryInfC{$\Gamma$, \textit{x}:(A$\times$B) $\vdash$ (snd \textit{x}):B}
\RightLabel{{\small $\times$Intro}}
\BinaryInfC{$\Gamma$, \textit{x}:(A$\times$B) $\vdash$ \{(snd \textit{x}),(fst \textit{x})\}:(B$\times$A)}
\RightLabel{{\small $\to$Intro}}
\UnaryInfC{$\emptyset$ $\vdash$ $\lambda$\textit{x}:(A$\times$B).\{(snd \textit{x}),(fst \textit{x})\}:((A$\times$B)$\to$(B$\times$A))}\end{prooftree}
Here is the cooresponding natural deduction proof:
\begin{prooftree}\RightLabel{{\small Ax}}
\AxiomC{(A$\land$B)}
\RightLabel{{\small $\land$Elim1}}
\UnaryInfC{A}
\RightLabel{{\small Ax}}
\AxiomC{(A$\land$B)}
\RightLabel{{\small $\land$Elim2}}
\UnaryInfC{B}
\RightLabel{{\small $\land$Intro}}
\BinaryInfC{(B$\land$A)}
\RightLabel{{\small $\to$Intro}}
\UnaryInfC{((A$\land$B)$\to$(B$\land$A))}\end{prooftree}

\hrule\vspace{1cm}
\noindent Here is a derivation of: $\lambda$\textit{x}\textsubscript{1}:(A+B).(case \textit{x}\textsubscript{1} of $\lambda$\textit{x}\textsubscript{2}:A.(inr \textit{x}\textsubscript{2} as (B+A)) $\vert$ $\lambda$\textit{x}\textsubscript{3}:B.(inl \textit{x}\textsubscript{3} as (B+A))):((A+B)$\to$(B+A))
\begin{prooftree}\RightLabel{{\small Ax}}
\AxiomC{$\Gamma$, \textit{x}\textsubscript{1}:(A+B), \textit{x}\textsubscript{3}:B $\vdash$ \textit{x}\textsubscript{3}:B}
\RightLabel{{\small +Intro2}}
\UnaryInfC{$\Gamma$, \textit{x}\textsubscript{1}:(A+B), \textit{x}\textsubscript{3}:B $\vdash$ (inl \textit{x}\textsubscript{3} as (B+A)):(B+A)}
\RightLabel{{\small $\to$Intro}}
\UnaryInfC{$\Gamma$, \textit{x}\textsubscript{1}:(A+B) $\vdash$ $\lambda$\textit{x}\textsubscript{3}:B.(inl \textit{x}\textsubscript{3} as (B+A)):(B$\to$(B+A))}
\RightLabel{{\small Ax}}
\AxiomC{$\Gamma$, \textit{x}\textsubscript{1}:(A+B), \textit{x}\textsubscript{2}:A $\vdash$ \textit{x}\textsubscript{2}:A}
\RightLabel{{\small +Intro1}}
\UnaryInfC{$\Gamma$, \textit{x}\textsubscript{1}:(A+B), \textit{x}\textsubscript{2}:A $\vdash$ (inr \textit{x}\textsubscript{2} as (B+A)):(B+A)}
\RightLabel{{\small $\to$Intro}}
\UnaryInfC{$\Gamma$, \textit{x}\textsubscript{1}:(A+B) $\vdash$ $\lambda$\textit{x}\textsubscript{2}:A.(inr \textit{x}\textsubscript{2} as (B+A)):(A$\to$(B+A))}
\RightLabel{{\small Ax}}
\AxiomC{$\Gamma$, \textit{x}\textsubscript{1}:(A+B) $\vdash$ \textit{x}\textsubscript{1}:(A+B)}
\RightLabel{{\small +Elim}}
\TrinaryInfC{$\Gamma$, \textit{x}\textsubscript{1}:(A+B) $\vdash$ (case \textit{x}\textsubscript{1} of $\lambda$\textit{x}\textsubscript{2}:A.(inr \textit{x}\textsubscript{2} as (B+A)) $\vert$ $\lambda$\textit{x}\textsubscript{3}:B.(inl \textit{x}\textsubscript{3} as (B+A))):(B+A)}
\RightLabel{{\small $\to$Intro}}
\UnaryInfC{$\emptyset$ $\vdash$ $\lambda$\textit{x}\textsubscript{1}:(A+B).(case \textit{x}\textsubscript{1} of $\lambda$\textit{x}\textsubscript{2}:A.(inr \textit{x}\textsubscript{2} as (B+A)) $\vert$ $\lambda$\textit{x}\textsubscript{3}:B.(inl \textit{x}\textsubscript{3} as (B+A))):((A+B)$\to$(B+A))}\end{prooftree}
Here is the cooresponding natural deduction proof:
\begin{prooftree}\RightLabel{{\small Ax}}
\AxiomC{B}
\RightLabel{{\small $\lor$Intro2}}
\UnaryInfC{(B$\lor$A)}
\RightLabel{{\small $\to$Intro}}
\UnaryInfC{(B$\to$(B$\lor$A))}
\RightLabel{{\small Ax}}
\AxiomC{A}
\RightLabel{{\small $\lor$Intro1}}
\UnaryInfC{(B$\lor$A)}
\RightLabel{{\small $\to$Intro}}
\UnaryInfC{(A$\to$(B$\lor$A))}
\RightLabel{{\small Ax}}
\AxiomC{(A$\lor$B)}
\RightLabel{{\small $\lor$Elim}}
\TrinaryInfC{(B$\lor$A)}
\RightLabel{{\small $\to$Intro}}
\UnaryInfC{((A$\lor$B)$\to$(B$\lor$A))}\end{prooftree}

\hrule\vspace{1cm}
\end{document}

